src/lib/data/Kuiper.Array1.fst
@@ -643,8 +643,23 @@ let ref_of_array_cell
   (#l : layout len)
   (a : array1 et l)
   (i : natlt len)
-  : ref et
-  = magic()
+  : GTot (ref et)
+  = Array.Core.ref_of_array_cell (core a) (l.imap.f (adapt_idx_back i))
+
+inline_for_extraction noextract
+fn get_ref_of_array_cell
+  (#et : Type0)
+  (#len : nat)
+  (#l : layout len) {| c : ctlayout l |}
+  (a : array1 et l)
+  (i : szlt len)
+  returns
+    r : ref et
+  ensures 
+    pure (r == ref_of_array_cell a i)
+{
+  Array.Core.get_ref_of_array_cell (core a) (c.cimap (i, ()))
+}
 
 ghost
 fn array1_cell_to_ref
@@ -653,13 +668,17 @@ fn array1_cell_to_ref
   (#l : layout len)
   (a : array1 et l)
   (i : natlt len)
+  (#f : perm)
   (#v : erased et)
   requires
-    Cell a i |-> v
+    Cell a i |-> Frac f v
   ensures
-    ref_of_array_cell a i |-> v
+    ref_of_array_cell a i |-> Frac f v
 {
-  admit();
+  pts_to_cell_eq a i f v;
+  rewrite Cell a i |-> Frac f v
+       as B.pts_to_cell (core a) #f (l.imap.f (adapt_idx_back i)) v;
+  Array.Core.array_cell_to_ref (core a) (l.imap.f (adapt_idx_back i));
 }
 
 ghost
@@ -669,11 +688,15 @@ fn array1_cell_from_ref
   (#l : layout len)
   (a : array1 et l)
   (i : natlt len)
+  (#f : perm)
   (#v : erased et)
   requires
-    ref_of_array_cell a i |-> v
+    ref_of_array_cell a i |-> Frac f v
   ensures
-    Cell a i |-> v
+    Cell a i |-> Frac f v
 {
-  admit();
+  pts_to_cell_eq a i f v;
+  Array.Core.array_cell_from_ref (core a) (l.imap.f (adapt_idx_back i));
+  rewrite B.pts_to_cell (core a) #f (l.imap.f (adapt_idx_back i)) v
+       as Cell a i |-> Frac f v;
 }
